@prefix rdf: <http://www.w3.org/1999/02/22-rdf-syntax-ns#> .
@prefix rdfs: <http://www.w3.org/2000/01/rdf-schema#> .
@prefix owl: <http://www.w3.org/2002/07/owl#> .
@prefix vann: <http://purl.org/vocab/vann/> .
@prefix ldp: <http://www.w3.org/ns/ldp#> .
@prefix vs: <http://www.w3.org/2003/06/sw-vocab-status/ns#> .
@prefix : <http://acdc.amherst.edu/ns/trellis#> .

: a owl:Ontology ;
    owl:versionInfo "0.1" ;
    vann:preferredNamespaceUri "http://acdc.amherst.edu/ns/trellis#";
    vann:preferredNamespacePrefix "trellis";
    rdfs:comment "Trellis Repository Ontology, Version 0.1" .

:PreferAudit a rdfs:Class ;
    rdfs:label "prefer audit" ;
    rdfs:comment "IRI identifying a LDPR's audit triples" ;
    rdfs:isDefinedBy : ;
    vs:term_status "working-draft" .

:ServerManagedTriples a rdfs:Class ;
    rdfs:label "server managed triples" ;
    rdfs:comment "IRI identifying a LDPR's server-managed triples" ;
    rdfs:isDefinedBy : ;
    vs:term_status "working-draft" .

:UserManagedTriples a rdfs:Class ;
    rdfs:label "user managed triples" ;
    rdfs:comment "IRI identifying a LDP-RS's user-managed resource triples" ;
    rdfs:isDefinedBy : ;
    vs:term_status "working-draft" .

:ConstraintViolation a rdfs:Class ;
    rdfs:label "constraint violation" ;
    rdfs:comment "A defined constraint was violated with the provided RDF graph" ;
    rdfs:isDefinedBy : ;
    vs:term_status "working-draft" .

:AccessViolation a rdfs:Class ;
    rdfs:label "access violation" ;
    rdfs:comment "The given operation (e.g. read, write, append) is not permitted to the provided user/group with regard to the specified resource(s)." ;
    rdfs:isDefinedBy : ;
    vs:term_status "working-draft" .

:DefaultInteractionModel a rdfs:Class ;
    rdfs:label "default interaction model" ;
    rdfs:comment "In the absence of a Link header defining an LDP interaction model, the implementation default will be assigned to the new resource." ;
    rdfs:isDefinedBy : ;
    vs:term_status "working-draft" .

:InvalidInteractionModel a rdfs:Class ;
    rdfs:label "invalid interaction model" ;
    rdfs:comment "An invalid LDP interaction model was provided" ;
    rdfs:subClassOf trellis:ConstraintViolation ;
    rdfs:isDefinedBy : ;
    vs:term_status "working-draft" .

:InvalidType a rdfs:Class ;
    rdfs:label "invalid type" ;
    rdfs:comment "An invalid rdf:type was included in the supplied graph, such as an invalid LDP resource type or a server-managed type." ;
    rdfs:subClassOf trellis:ConstraintViolation ;
    rdfs:isDefinedBy : ;
    vs:term_status "working-draft" .

:InvalidCardinality a rdfs:Class ;
    rdfs:label "invalid cardinality" ;
    rdfs:comment "For properties with cardinality restrictions, the supplied graph did not correspond to the defined rules regarding cardinality." ;
    rdfs:subClassOf trellis:ConstraintViolation ;
    rdfs:isDefinedBy : ;
    vs:term_status "working-draft" .

:InvalidRange a rdfs:Class ;
    rdfs:label "invalid range" ;
    rdfs:comment "For properties with range constraints (e.g. IRI or in-domain ranges), the supplied graph violated these constraints." ;
    rdfs:subClassOf trellis:ConstraintViolation ;
    rdfs:isDefinedBy : ;
    vs:term_status "working-draft" .

:InvalidProperty a rdfs:Class ;
    rdfs:label "invalid property" ;
    rdfs:comment "LDP interaction models permit certain valid properties; the supplied graph did not conform to the defined rules for an allowable property." ;
    rdfs:subClassOf trellis:ConstraintViolation ;
    rdfs:isDefinedBy : ;
    vs:term_status "working-draft" .

:containedBy a rdf:Property ;
    rdfs:label "contained by" ;
    rdfs:comment "Links a resource to the container resource that encloses it." ;
    rdfs:domain ldp:Resource ;
    rdfs:range ldp:Container ;
    rdfs:isDefinedBy : ;
    owl:inverseOf ldp:contains ;
    vs:term_status "working-draft" .

